src/Pyrosome/Lang/CombinedThm.v
@@ -6,9 +6,12 @@ Import ListNotations.
 Open Scope string.
 Open Scope list.
 From Utils Require Import Utils.
-From Named Require Import Core Compilers Elab ElabCompilers
-     SimpleVSubst SimpleVCPS SimpleEvalCtx SimpleEvalCtxCPS SimpleUnit NatHeap SimpleVCPSHeap
-     SimpleVFixCPS SimpleVFixCC SimpleVCC SimpleVSTLC SimpleVCCHeap SimpleVFix Matches CompilerTransitivity CompilerTools.
+From Pyrosome Require Import Theory.Core Compilers.Compilers Elab.Elab Elab.ElabCompilers
+  Tools.Matches Tools.CompilerTools.
+From Pyrosome.Lang Require Import SimpleVSubst SimpleVCPS SimpleEvalCtx SimpleEvalCtxCPS
+  SimpleUnit NatHeap SimpleVCPSHeap
+  SimpleVFixCPS SimpleVFixCC SimpleVCC SimpleVSTLC SimpleVCCHeap SimpleVFix.
+(*TODO: fix these or replace them CompilerTransitivity CompilerTools.*)
 Import Core.Notations.
 (*TODO: repackage this in compilers*)
 Import CompilerDefs.Notations.
@@ -16,41 +19,30 @@ Import CompilerDefs.Notations.
 Require Coq.derive.Derive.
 
 
-Local Notation compiler_case := (compiler_case string).
+Local Notation compiler_case := (compiler_case string (tgt_term:=term) (tgt_sort:=sort)).
 
 (*TODO: put in right place*)
 
-Import SumboolNotations.
+(*TODO: move to compilerdefs.v*)
+#[export] Instance compiler_case_Eqb : Eqb compiler_case :=
+  fun c1 c2 =>
+    match c1, c2 with
+    | sort_case args t, sort_case args' t' =>
+        (eqb args args') && (eqb t t')
+    | term_case args t, term_case args' t' =>
+        (eqb args args') && (eqb t t')
+    | _,_ => false
+    end%bool.
 
-Definition case_eq_dec (r1 r2 : compiler_case) : {r1 = r2} + {~ r1 = r2}.
-  refine(match r1, r2 with
-         | sort_case args t, sort_case args' t' =>
-           SB! (list_eq_dec string_dec args args') SB&
-           (sort_eq_dec t t')
-         | term_case args t, term_case args' t' =>
-           SB! (list_eq_dec string_dec args args') SB&
-           (term_eq_dec t t')
-         | _,_ => _
-         end); autorewrite with utils lang_core; try intuition fail.
-  all: try typeclasses eauto.
-  all: right.
-  all: intros; basic_core_crush.
-Defined.
-
-Definition compute_incl_compiler (l1 l2 : compiler) :=
-  if incl_dec (pair_eq_dec string_dec case_eq_dec) l1 l2 then true else false.
-
-Lemma use_compute_incl_compiler l1 l2
-  : compute_incl_compiler l1 l2 = true -> incl l1 l2.
+#[export] Instance compiler_case_Eqb_ok : Eqb_ok compiler_case_Eqb.
 Proof.
-  unfold compute_incl_compiler.
-  destruct (incl_dec _ l1 l2); easy.
+  intros a b;
+    destruct a, b;
+    cbn [eqb compiler_case_Eqb];
+    try congruence.
+  all: case_match;
+    basic_core_crush.
 Qed.
-
-Ltac solve_incl := 
-  solve [basic_utils_crush
-        | eapply use_compute_incl_compiler; vm_compute; reflexivity
-        | eapply use_compute_incl_lang; vm_compute; reflexivity].
 (*
 
 Lemma elab_preserving_compiler_monotonicity cmp' cmp_pre tgt cmp ecmp src src_pre cmp_pre'
@@ -77,20 +69,20 @@ Hint Resolve fix_cps_preserving : elab_pfs.
 Hint Resolve ElabCompilers.elab_preserving_compiler_nil : auto_elab.
 
 
-Lemma preserving_compiler_embed cmp_pre tgt cmp src tgt'
-    : preserving_compiler_ext cmp_pre tgt cmp src ->
+Lemma preserving_compiler_embed {V} `{Eqb_ok V} `{WithDefault V} cmp_pre (tgt : Rule.lang V) cmp src tgt'
+    : preserving_compiler_ext (tgt_Model:=core_model tgt) cmp_pre cmp src ->
       incl tgt tgt' ->
-      preserving_compiler_ext cmp_pre tgt' cmp src.
+      preserving_compiler_ext (tgt_Model:=core_model tgt') cmp_pre cmp src.
 Proof.
   induction 1; basic_goal_prep; constructor; basic_core_firstorder_crush.
-  eapply wf_sort_lang_monotonicity; eauto.
-  eapply wf_term_lang_monotonicity; eauto.
-  eapply eq_sort_lang_monotonicity; eauto.
-  eapply eq_term_lang_monotonicity; eauto.
+  - eapply wf_sort_lang_monotonicity; eauto.
+  - eapply wf_term_lang_monotonicity; eauto.
+  - eapply eq_sort_lang_monotonicity; eauto.
+  - eapply eq_term_lang_monotonicity; eauto.
 Qed.
 Hint Resolve preserving_compiler_embed : auto_elab.
 
-Require Import AllConstructors.
+Require Import Pyrosome.Tools.AllConstructors.
 
 Hint Resolve incl_nil_l : utils.
 Lemma incl_map_first {A B} (a b : list (A * B))
@@ -103,67 +95,76 @@ Proof.
     basic_utils_crush.
 Qed.
 
-Lemma elab_compiler_prefix_implies_elab cmp_pre target cmp src src_pre
-    : preserving_compiler_ext [] target cmp_pre src_pre ->
-      preserving_compiler_ext cmp_pre target cmp src ->
-      preserving_compiler_ext [] target (cmp++cmp_pre) (src++src_pre).
+Lemma elab_compiler_prefix_implies_elab {V} `{Eqb_ok V} `{WithDefault V} cmp_pre (target : Rule.lang V)
+  cmp src src_pre
+    : preserving_compiler_ext (tgt_Model:=core_model target) [] cmp_pre src_pre ->
+      preserving_compiler_ext (tgt_Model:=core_model target) cmp_pre cmp src ->
+      preserving_compiler_ext (tgt_Model:=core_model target) [] (cmp++cmp_pre) (src++src_pre).
   Proof using.
     induction 2; basic_goal_prep; basic_core_firstorder_crush.
     all: constructor; basic_core_crush.
   Qed.
 
-Lemma preserving_compiler_monotonicity cmp_pre tgt cmp src src_pre cmp_pre'
-  : preserving_compiler_ext [] tgt cmp_pre src_pre ->
-    preserving_compiler_ext cmp_pre tgt cmp src ->
+  Lemma preserving_compiler_monotonicity {V} `{Eqb_ok V} `{WithDefault V} cmp_pre
+    (tgt : Rule.lang V) cmp src src_pre cmp_pre'
+  : preserving_compiler_ext (tgt_Model:=core_model tgt) [] cmp_pre src_pre ->
+    preserving_compiler_ext (tgt_Model:=core_model tgt) cmp_pre cmp src ->
     wf_lang (src++src_pre) ->
     incl cmp_pre cmp_pre' ->
     all_fresh cmp_pre' ->
-    preserving_compiler_ext cmp_pre' tgt cmp src.
+    preserving_compiler_ext (tgt_Model:=core_model tgt) cmp_pre' cmp src.
 Proof.
   induction 2; basic_goal_prep; autorewrite with utils lang_core in *;
     try typeclasses eauto; try constructor; intuition eauto.
+  
+  all: unfold Model.wf_sort, Model.wf_term, Model.eq_sort, Model.eq_term, core_model.
   Ltac solve_sort_goal :=
-      eapply all_constructors_sort_weaken; [typeclasses eauto|..]; cycle 1;
-      [eapply all_constructors_sort_from_wf; eauto|];
+    eapply all_constructors_sort_weaken;
+    [typeclasses eauto|typeclasses eauto|..]; cycle 1;
+      [eapply all_constructors_sort_from_wf; eauto using core_model |];
       simpl; intro;
       erewrite !preserving_compiler_constructor_names; eauto;
         eapply elab_compiler_prefix_implies_elab; eauto.
   Ltac solve_ctx_goal :=
-      eapply all_constructors_ctx_weaken; [typeclasses eauto|..]; cycle 1;
-      [eapply all_constructors_ctx_from_wf; eauto|];
+      eapply all_constructors_ctx_weaken; [typeclasses eauto |typeclasses eauto|..]; cycle 1;
+      [eapply all_constructors_ctx_from_wf; eauto using core_model|];
       simpl; intro;
       erewrite !preserving_compiler_constructor_names; eauto;
-        eapply elab_compiler_prefix_implies_elab; eauto.
-  all: erewrite ?compile_strengthen_ctx_incl' by (eauto;solve_ctx_goal); auto.
-  all: erewrite ?compile_strengthen_sort_incl' by (eauto;solve_sort_goal); auto.
-  all: erewrite ?(compile_strengthen_sort_incl' _ t2) by (eauto;solve_sort_goal); auto.
+      eapply elab_compiler_prefix_implies_elab; eauto.
+  
+  all: erewrite ?compile_strengthen_ctx_incl'
+    by (try typeclasses eauto; eauto using core_model;solve_ctx_goal); auto.
+  all: erewrite !compile_strengthen_sort_incl' with (cmp':=cmp_pre')
+      by (try typeclasses eauto; eauto using core_model;solve_sort_goal); auto.
   Ltac solve_term_goal :=
-      eapply all_constructors_term_weaken; [typeclasses eauto|..]; cycle 1;
-      [eapply all_constructors_term_from_wf; eauto|];
+    eapply all_constructors_term_weaken;
+    [typeclasses eauto|typeclasses eauto|..]; cycle 1;
+      [eapply all_constructors_term_from_wf; eauto using core_model |];
       simpl; intro;
       erewrite !preserving_compiler_constructor_names; eauto;
-        eapply elab_compiler_prefix_implies_elab; eauto.
-  erewrite ?compile_strengthen_term_incl' by (eauto;solve_term_goal); auto.
-  erewrite (compile_strengthen_term_incl' _ e2) by (eauto;solve_term_goal); auto.
-Qed.
+    eapply elab_compiler_prefix_implies_elab; eauto.
+
+  erewrite !compile_strengthen_term_incl' with (cmp':=cmp_pre')
+      by (try typeclasses eauto; eauto using core_model;solve_term_goal); auto.
+Qed.  
 
   
-Lemma compiler_append cmp_pre' lt' cmp' ls' lt cmp ls src_pre'
-  : preserving_compiler_ext cmp_pre' lt' cmp' ls' ->
-    preserving_compiler_ext [] lt cmp_pre' src_pre' ->
-    preserving_compiler_ext [] lt cmp ls ->
+Lemma compiler_append {V} `{Eqb_ok V} `{WithDefault V}
+  cmp_pre' lt' cmp' (ls' : Rule.lang V) lt cmp ls src_pre'
+  : preserving_compiler_ext (tgt_Model:=core_model lt') cmp_pre' cmp' ls' ->
+    preserving_compiler_ext (tgt_Model:=core_model lt) [] cmp_pre' src_pre' ->
+    preserving_compiler_ext (tgt_Model:=core_model lt) [] cmp ls ->
     incl lt' lt ->
     incl cmp_pre' cmp ->
     all_fresh cmp ->
     wf_lang (ls' ++ src_pre') ->
-    preserving_compiler_ext [] lt (cmp' ++ cmp) (ls' ++ ls).
+    preserving_compiler_ext (tgt_Model:=core_model lt) [] (cmp' ++ cmp) (ls' ++ ls).
 Proof.
   intros.
-  eapply preserving_compiler_embed in H; eauto.
-  clear lt' H2.
+  eapply preserving_compiler_embed in H2; [| eassumption].
   eapply elab_compiler_prefix_implies_elab; auto.
   eapply preserving_compiler_monotonicity.
-  exact H0.
+  1:exact H3.
   all: eauto.
 Qed.
   
@@ -174,7 +175,7 @@ Ltac solve_compiler_lookup :=
             | shelve].
   
 
-Lemma wf_lang_concat l l1 l2
+Lemma wf_lang_concat {V} `{Eqb_ok V} `{WithDefault V} (l : Rule.lang V) l1 l2
   : wf_lang_ext l l1 ->
     wf_lang_ext (l1 ++ l) l2 ->
     wf_lang_ext l (l2 ++ l1).
@@ -184,20 +185,17 @@ Proof.
 Qed.
 Hint Resolve wf_lang_concat : lang_core.
 
-(*TODO: this is still a tactic performance bottleneck;
-  reduce number of calls to it
- *)
-Ltac prove_from_known_elabs ::=
-  (*TODO: is this what I want, or something more general?*)
+(*TODO: duplicated; backport above lemma*)
+Ltac prove_from_known_elabs :=
   rewrite <- ?as_nth_tail;
-  repeat
+   repeat
     lazymatch goal with
     | |- wf_lang_ext ?l_pre (?l1 ++ ?l2) => apply wf_lang_concat
+    | |- wf_lang_ext _ [] => apply wf_lang_nil
     | |- wf_lang_ext _ _ => prove_ident_from_known_elabs
-    | |- all_fresh _ => apply use_compute_all_fresh; vm_compute; reflexivity
-    | |- incl _ _ => simple eapply use_compute_incl_lang; compute; reflexivity
+    | |- all_fresh _ => compute_all_fresh
+    | |- incl _ _ => compute_incl
     end.
-
 
 Ltac build_compiler :=  
   unshelve(repeat (first [apply preserving_compiler_nil
@@ -205,15 +203,15 @@ Ltac build_compiler :=
                          | solve_compiler_lookup
                          | shelve]));
   first [apply incl_refl
-        |eapply use_compute_all_fresh; compute; reflexivity
-        |solve_incl
+        |compute_all_fresh
+        |compute_incl
         |prove_from_known_elabs].
 
 
 (*TODO: add let*)
 Lemma full_cps_compiler_preserving
-  : preserving_compiler_ext []
-      (heap_cps_ops
+  : preserving_compiler_ext
+      (tgt_Model := core_model (heap_cps_ops
          ++ fix_cps_lang
          ++ cps_lang
          ++ cps_prod_lang
@@ -222,31 +220,36 @@ Lemma full_cps_compiler_preserving
          ++ nat_exp
          ++ nat_lang
          ++ block_subst
-         ++ value_subst)
+         ++ value_subst))
+      []
       (fix_cps++ cps ++ heap_ctx_cps ++ Ectx_cps++ heap_cps++heap_id++cps_subst++[])
       (SimpleVFix.fix_lang++SimpleVSTLC.stlc++ heap_ctx++ eval_ctx++heap_ops++(unit_lang ++ heap ++ nat_exp ++ nat_lang)++(exp_subst ++ value_subst)++[]).
-Proof.  build_compiler. Qed.
+Proof. build_compiler. Qed.
 
 
 Lemma full_cc_compiler_preserving
-  : preserving_compiler_ext [] (fix_cc_lang ++
+  : preserving_compiler_ext
+      (tgt_Model := core_model (fix_cc_lang ++
      heap_cps_ops ++cc_lang ++ forget_eq_wkn ++ unit_eta ++ unit_lang
                                       ++ heap ++ nat_exp ++ nat_lang ++ prod_cc ++
                                       forget_eq_wkn'++
-                                      cps_prod_lang ++ block_subst ++ value_subst)
+                                      cps_prod_lang ++ block_subst ++ value_subst))
+      []
                         (fix_cc++heap_cc++heap_id'++cc++prod_cc_compile++subst_cc++[])
                         (fix_cps_lang++heap_cps_ops++(unit_lang ++ heap ++ nat_exp ++ nat_lang)
                             ++cps_lang++cps_prod_lang++(block_subst ++ value_subst)++[]).
 Proof. build_compiler. Qed.
 
 
-
+(*TODO: compiler transitivity*)
 Lemma full_compiler_preserving
-  : preserving_compiler_ext [] (fix_cc_lang ++
+  : preserving_compiler_ext
+      (tgt_Model := core_model (fix_cc_lang ++
                                      heap_cps_ops ++cc_lang ++ forget_eq_wkn ++ unit_eta ++ unit_lang
                                      ++ heap ++ nat_exp ++ nat_lang ++ prod_cc ++
                                      forget_eq_wkn'++
-                                     cps_prod_lang ++ block_subst ++ value_subst)
+                                     cps_prod_lang ++ block_subst ++ value_subst))
+      []
                         (compile_cmp (fix_cc++heap_cc++heap_id'++cc++prod_cc_compile++subst_cc++[])
                         (fix_cps++ cps ++ heap_ctx_cps ++ Ectx_cps++ heap_cps++heap_id++cps_subst++[]))
       (SimpleVFix.fix_lang++SimpleVSTLC.stlc++ heap_ctx++ eval_ctx++heap_ops++(unit_lang ++ heap ++ nat_exp ++ nat_lang)++(exp_subst ++ value_subst)++[]).
